approach.thy
@@ -16,6 +16,119 @@ TODO:
 *)
 
 
+declare length_dropWhile_le[simp]  
+  
+(*
+split a trace into maximal chunks of actions in the same session.
+Each chunk can be used in single-session semantics.
+
+Remember that a trace is just a (session\<times>action) list
+*)
+fun split_trace :: "trace \<Rightarrow> (session \<times> (action list)) list" where
+  "split_trace [] = []"
+| "split_trace ((s,a)#rest) = (
+   let same = map snd (takeWhile (\<lambda>x. fst x = s) rest);
+       rest' = dropWhile (\<lambda>x. fst x = s) rest
+   in (s, a#same) # split_trace rest'
+)"
+
+term steps_s
+
+lemma 
+fixes tr :: trace
+  and s :: session      
+  and S S' :: state
+assumes steps: "S ~~ tr \<leadsto>* S'"
+    and singleSession: "\<And>a. a\<in>set tr \<Longrightarrow> fst a = s"
+    and inv: "invariant (prog S) (invContext init s)"
+shows "\<exists>tr' S'' a.  (S ~~ (s, tr') \<leadsto>\<^sub>S* S'') 
+        \<and> ((s, AInvcheck False) \<in> set tr \<longrightarrow>  (a, False)\<in>set tr')
+        \<and> S'' = S'" (* TODO instead S'' = S' maybe some weaker coupling relation here*)
+using steps singleSession proof (induct rule: steps.induct)
+  case (steps_refl S)
+  then show ?case
+    using steps_s.steps_refl by auto
+next
+  case (steps_step S tr S' a S'')
+  hence  steps: "S ~~ tr \<leadsto>* S'"
+    and  IH: "\<lbrakk>\<And>a. a \<in> set tr \<Longrightarrow> fst a = s\<rbrakk>
+        \<Longrightarrow> \<exists>tr' S'' a. 
+              (S ~~ (s, tr') \<leadsto>\<^sub>S* S'') 
+            \<and> ((s, AInvcheck False) \<in> set tr \<longrightarrow> (a, False) \<in> set tr') 
+            \<and> S'' = S'"
+    and  step: "S' ~~ a \<leadsto> S''"
+    and  singleSession: "\<And>a'. a' \<in> set (tr @ [a]) \<Longrightarrow> fst a' = s"
+    by auto
+ 
+   
+    
+  show ?case 
+  proof (cases "snd a")
+    case ALocal
+    hence "a = (s, ALocal)"
+      by (simp add: prod.expand singleSession) 
+
+    with step
+    have step': "S' ~~ (s, ALocal) \<leadsto> S''" by simp
+    
+    from step_elim_ALocal[OF step']
+    obtain ls f ls' 
+       where a1: "S'' = S'\<lparr>localState := localState S'(s \<mapsto> ls')\<rparr>"
+         and a2: "localState S' s \<triangleq> ls"
+         and a3: "currentProc S' s \<triangleq> f"
+         and a4: "f ls = LocalStep ls'"
+       by metis
+    
+    from a2 a3 a4
+    have step_s: "S' ~~ (s,(ALocal,True)) \<leadsto>\<^sub>S S'\<lparr>localState := localState S'(s \<mapsto> ls')\<rparr>"
+      by (rule step_s.local)
+    
+    from IH obtain tr' S''_s a_s
+      where ih1: "S ~~ (s, tr') \<leadsto>\<^sub>S* S''_s"
+        and ih2: "(s, AInvcheck False) \<in> set tr \<longrightarrow> (a_s, False) \<in> set tr'"
+        and ih3: "S''_s = S'"
+      using singleSession by auto
+        
+      
+    hence "S ~~ (s, tr') \<leadsto>\<^sub>S* S''"
+    
+    then show ?thesis sorry
+  next
+    case (ANewId x2)
+    then show ?thesis sorry
+  next
+    case (ABeginAtomic x3)
+    then show ?thesis sorry
+  next
+    case AEndAtomic
+    then show ?thesis sorry
+  next
+    case (ADbOp x51 x52 x53 x54)
+    then show ?thesis sorry
+  next
+    case (APull x6)
+    then show ?thesis sorry
+  next
+    case (AInvoc x71 x72)
+    then show ?thesis sorry
+  next
+    case (AReturn x8)
+    then show ?thesis sorry
+  next
+    case AFail
+    then show ?thesis sorry
+  next
+    case (AInvcheck x10)
+    then show ?thesis sorry
+  qed
+    
+    
+  
+  qed
+qed
+
+
+
 
 text {*
 When a program is correct in the single session semantics, 
